@prefix owl: <http://www.w3.org/2002/07/owl#> .
@prefix prof: <http://www.w3.org/ns/dx/prof/> .
@prefix profrole: <http://www.w3.org/ns/dx/prof/role/> .
@prefix profiles: <http://www.opengis.net/def/metamodel/profiles/> .
@prefix rdf: <http://www.w3.org/1999/02/22-rdf-syntax-ns#> .
@prefix rdfs: <http://www.w3.org/2000/01/rdf-schema#> .
@prefix xsd: <http://www.w3.org/2001/XMLSchema#> .
@prefix dct: <http://purl.org/dc/terms/> .
@prefix skos: <http://www.w3.org/2004/02/skos/core#> .
@prefix jsonld:  <https://www.w3.org/TR/json-ld/> .
@prefix jsoncontext: <http://www.opengis.net/def/metamodel/profiles/json_ld_context> .



profiles:ogcapi
  a   skos:Concept ;
  skos:definition "OGC API family of APIs and building blocks.";

  rdfs:comment "Initial thoughts on how to describe the relations between these" ;
  skos:prefLabel "OGC API Suite"@en ;
  prof:hasToken "ogcapi"^^xsd:token ;
  skos:inScheme <http://www.opengis.net/def/metamodel/profiles> ;
  skos:narrower profiles:ogcapi-common, profiles:ogcapi-blocks ;
  skos:topConceptOf <http://www.opengis.net/def/metamodel/profiles> ;
  
.

profiles:ogcapi-blocks
  a   skos:Concept ;
  skos:definition "OGC API building blocks.";

  rdfs:comment "Initial thoughts on how to describe the relations between these" ;
  skos:prefLabel "OGC API Building Blocks"@en ;
  prof:hasToken "ogcapi"^^xsd:token ;
  skos:inScheme <http://www.opengis.net/def/metamodel/profiles> ;
  
.

profiles:ogcapi-common
  a   skos:Concept , dct:Standard, prof:Profile ;
  skos:definition "OGC API common.";

  rdfs:comment "Initial thoughts on how to describe the relations between these" ;
  skos:prefLabel "OGC API Common"@en ;
  prof:hasToken "ogcapi"^^xsd:token ;
  skos:inScheme <http://www.opengis.net/def/metamodel/profiles> ;
  
.

profiles:ogcapi-features
  a   skos:Concept , dct:Standard, prof:Profile ;
  skos:definition "OGC API Features.";

  rdfs:comment "Initial thoughts on how to describe the relations between these" ;
  skos:prefLabel "OGC API Features"@en ;
  prof:hasToken "ogcapi-features"^^xsd:token ;
  prof:isProfileOf profiles:ogcapi-common ;
  skos:inScheme <http://www.opengis.net/def/metamodel/profiles> ;
  
.

profiles:ogcapi-edr
  a   skos:Concept , dct:Standard, prof:Profile ;
  skos:definition "OGC API Environmental Data Retrieval.";

  rdfs:comment "Initial thoughts on how to describe the relations between these" ;
  skos:prefLabel "OGC API EDR (Environmental Data Retrieval)"@en ;
  prof:hasToken "ogcapi-edr"^^xsd:token ;
  skos:inScheme <http://www.opengis.net/def/metamodel/profiles> ;
  prof:isProfileOf profiles:ogcapi-features ;
  
.

profiles:ogcapi-bbox
  a   skos:Concept , dct:Standard, prof:Profile ;
  skos:definition "Bounding Box - a reusable building block for OGC API data schemas";

  rdfs:comment "Initial thoughts on how to describe the relations between these" ;
  skos:prefLabel "Bounding Box"@en ;
  prof:hasToken "ogcapi-bbox"^^xsd:token ;
  skos:inScheme <http://www.opengis.net/def/metamodel/profiles> ;
  skos:broader profiles:ogcapi-blocks ;
  
.

profiles:ogcapi-geopose
  a   skos:Concept , dct:Standard, prof:Profile ;
  skos:definition "Geopose - a reusable building block for OGC API data schemas";

  rdfs:comment "Initial thoughts on how to describe the relations between these" ;
  skos:prefLabel "Geopose"@en ;
  prof:hasToken "ogcapi-geopose"^^xsd:token ;
  skos:inScheme <http://www.opengis.net/def/metamodel/profiles> ;
  skos:broader profiles:ogcapi-blocks ;
  prof:hasResource 
  		[ a prof:ResourceDescriptor ;
            rdfs:label "Geopose JSON schema (Advanced)" ;
            dct:format "application/json" ;
            prof:hasArtifact <https://schemas.opengis.net/geopose/1.0/schemata/GeoPose.Advanced.Schema.json> ;
            prof:hasRole profrole:schema 
            ] ;
  
.

profiles:ogcapi-geopose-euler
  a   skos:Concept , dct:Standard, prof:Profile ;
  skos:definition "Basic-Euler: Basic GeoPose using Euler angle rotations to specify orientation";

  rdfs:comment "Initial thoughts on how to describe the relations between these" ;
  skos:prefLabel "Geopose (Basic Euler)"@en ;
  prof:hasToken "ogcapi-geopose-euler"^^xsd:token ;
  skos:inScheme <http://www.opengis.net/def/metamodel/profiles> ;
  skos:broader profiles:ogcapi-geopose ;
  prof:hasResource 
  		[ a prof:ResourceDescriptor ;
            rdfs:label "Geopose JSON schema (Advanced)" ;
            dct:format "application/json" ;
            prof:hasArtifact <https://schemas.opengis.net/geopose/1.0/schemata/GeoPose.Basic.Euler.Schema.json> ;
            prof:hasRole profrole:schema 
            ] ;
  
.








